wip on correctness

NLustreToSyMac/Correctness.v
@@ -35,6 +35,22 @@ Module Type CORRECTNESS
        (Import Mem   : MEMORIES    Ids Op       Clks SynNL)
        (Import Trans : TRANSLATION Ids Op       Clks SynNL SynSM Mem).
 
+  Fixpoint memvar_lexp (x: ident) (e: SynSM.lexp) :=
+    match e with
+    | SynSM.Emem y _ => x = y
+    | SynSM.Ewhen e _ _ => memvar_lexp x e
+    | SynSM.Eunop _ e _ => memvar_lexp x e
+    | SynSM.Ebinop _ e1 e2 _ => memvar_lexp x e1 \/ memvar_lexp x e2
+    | _ => False
+    end.
+
+  Fixpoint memvar_cexp (x: ident) (ce: SynSM.cexp) :=
+    match ce with
+    | SynSM.Emerge _ e1 e2 => memvar_cexp x e1 \/ memvar_cexp x e2
+    | SynSM.Eite e t f => memvar_lexp x e \/ memvar_cexp x t \/ memvar_cexp x f
+    | SynSM.Eexp e => memvar_lexp x e
+    end.
+
   Definition memory_spec (m: SemSM.memory) (memids: PS.t) (R: env) :=
     forall x v,
       PM.find x R = Some v ->
@@ -73,7 +89,6 @@ Module Type CORRECTNESS
 
       Variable m: SemSM.memory.
       Variable memids: PS.t.
-      Hypothesis Spec: memory_spec m memids R.
       (* Variable mems: list (ident * const). *)
       (* Let memids := ps_from_list (map fst mems). *)
 
@@ -85,6 +100,8 @@ Module Type CORRECTNESS
         destruct (PS.mem i memids); auto.
       Qed.
       (* Hint Resolve typeof_correctness. *)
+
+      Hypothesis Spec: memory_spec m memids R.
 
       Lemma lexp_instant_correctness:
         forall e v,
@@ -122,10 +139,75 @@ Module Type CORRECTNESS
         induction 1; simpl; eauto using SemSM.sem_cexp_instant.
       Qed.
 
+      Lemma sem_lexp_instant_madd_mem:
+        forall x mv e v,
+          SemSM.sem_lexp_instant base R m e v ->
+          ~ memvar_lexp x e ->
+          SemSM.sem_lexp_instant base R (madd_mem x mv m) e v.
+      Proof.
+        induction 1; simpl; intros Nmv; eauto using SemSM.sem_lexp_instant.
+        - do 2 constructor.
+          match goal with H: SemSM.sem_mem_var_instant _ _ _ |- _ => inv H end.
+          unfold SemSM.get_mem in *.
+          rewrite mfind_mem_gso; auto.
+        - econstructor; eauto.
+        - econstructor; eauto.
+      Qed.
+      Hint Resolve sem_lexp_instant_madd_mem.
+
+      Lemma sem_cexp_instant_madd_mem:
+        forall x mv ce v,
+          SemSM.sem_cexp_instant base R m ce v ->
+          ~ memvar_cexp x ce ->
+          SemSM.sem_cexp_instant base R (madd_mem x mv m) ce v.
+      Proof.
+        induction 1; simpl; intros Nmv; eauto using SemSM.sem_cexp_instant.
+        - econstructor; eauto.
+        - econstructor 2; eauto.
+        - econstructor; eauto.
+        - econstructor; eauto.
+          + apply IHsem_cexp_instant1; auto.
+          + apply IHsem_cexp_instant2; auto.
+        - econstructor; eauto.
+          + apply IHsem_cexp_instant1; auto.
+          + apply IHsem_cexp_instant2; auto.
+      Qed.
+
+      Lemma sem_lexps_instant_madd_mem:
+        forall x mv es vs,
+          SemSM.sem_lexps_instant base R m es vs ->
+          Forall (fun e => ~ memvar_lexp x e) es ->
+          SemSM.sem_lexps_instant base R (madd_mem x mv m) es vs.
+      Proof.
+        induction 1; simpl; intros Nmv; inv Nmv.
+        - constructor.
+        - constructor; auto.
+          apply IHForall2; auto.
+      Qed.
+
     End SemInstant.
     Hint Resolve var_instant_correctness clock_instant_correctness
          lexp_instant_correctness lexps_instant_correctness
-         cexp_instant_correctness.
+         cexp_instant_correctness
+         sem_cexp_instant_madd_mem sem_lexps_instant_madd_mem.
+
+    Lemma pm_map_add:
+      forall {A B} (m: PM.t A) (f: A -> B) x v,
+        PM.map f (PM.add x v m) = PM.add x (f v) (PM.map f m).
+    Proof.
+    Admitted.
+
+    Lemma restr_mem_madd_mem:
+      forall x mvs M n,
+        SemSM.restr_mem (madd_mem x mvs M) n =
+        madd_mem x (SemSM.restr_mvalues n mvs) (SemSM.restr_mem M n).
+    Proof.
+      intros.
+      unfold SemSM.restr_mem, madd_mem; simpl.
+      f_equal.
+      - now rewrite pm_map_add, mm_values_map.
+      - now rewrite mm_instances_map.
+    Qed.
 
     Section Sem.
 
@@ -179,8 +261,7 @@ Module Type CORRECTNESS
           sem_laexps bk H ck es vs ->
           SemSM.sem_laexps bk H M ck (map (translate_lexp memids) es) vs.
       Proof.
-        intros ** Sem n; specialize (Sem n); simpl in Sem.
-        induction Sem.
+        intros ** Sem n; specialize (Sem n); inv Sem.
         - econstructor 1; eauto.
         - constructor; auto.
           now rewrite all_absent_map.
@@ -197,10 +278,82 @@ Module Type CORRECTNESS
         - induction Sem; repeat constructor; auto.
       Qed.
 
+      Lemma sem_caexp_madd_mem:
+        forall x mvs ck ce xs,
+          SemSM.sem_caexp bk H M ck ce xs ->
+          ~ memvar_cexp x ce ->
+          SemSM.sem_caexp bk H (madd_mem x mvs M) ck ce xs.
+      Proof.
+        intros ** Sem ? n; specialize (Sem n); inv Sem;
+          econstructor; eauto;
+            rewrite restr_mem_madd_mem; auto.
+      Qed.
+
+      Lemma sem_laexps_madd_mem:
+        forall x mvs ck es xss,
+          SemSM.sem_laexps bk H M ck es xss ->
+          Forall (fun e => ~ memvar_lexp x e) es ->
+          SemSM.sem_laexps bk H (madd_mem x mvs M) ck es xss.
+      Proof.
+        intros ** Sem ? n; specialize (Sem n); inv Sem.
+        - econstructor; eauto.
+          rewrite restr_mem_madd_mem; auto.
+        - econstructor 2; eauto.
+          rewrite restr_mem_madd_mem; auto.
+        - constructor 3.
+      Qed.
+
+      Lemma sem_equation_madd_mem:
+        forall x mvs mems k eqs,
+          (* ~Is_defined_in_eqs x eqs -> *)
+          Forall (SemSM.sem_equation P k bk H M mems) eqs ->
+          Forall (SemSM.sem_equation P k bk H (madd_mem x mvs M) mems) eqs.
+      Proof.
+        intros ** (* Hnd *) Hsem.
+        induction eqs as [|eq eqs IH]; [now constructor|].
+        (* apply not_Is_defined_in_cons in Hnd. *)
+        (* destruct Hnd as [Hnd Hnds]. *)
+        apply Forall_cons2 in Hsem as [Hsem Hsems].
+        constructor; auto.
+        destruct Hsem; eauto using SemSM.sem_equation.
+        - econstructor; eauto.
+          apply sem_caexp_madd_mem; auto.
+          admit.
+        - admit.
+        - econstructor; eauto.
+          apply sem_laexps_madd_mem; auto.
+          admit.
+      Admitted.
+
     End Sem.
     Hint Resolve var_correctness vars_correctness
          laexp_correctness caexp_correctness laexps_correctness.
 
+
+  Lemma msem_equation_madd_obj:
+    forall G bk H M M' x eqs,
+      ~Is_defined_in_eqs x eqs ->
+      Forall (msem_equation G bk H M) eqs ->
+      Forall (msem_equation G bk H (add_objs x M' M)) eqs.
+  Proof.
+    Hint Constructors msem_equation.
+    intros * Hnd Hsem.
+    induction eqs as [|eq eqs IH]; [now constructor|].
+    apply not_Is_defined_in_cons in Hnd.
+    destruct Hnd as [Hnd Hnds].
+    apply Forall_cons2 in Hsem.
+    destruct Hsem as [Hsem Hsems].
+    constructor; [|now apply IH with (1:=Hnds) (2:=Hsems)].
+    destruct Hsem as [|??? x' ??????? Hsome
+                         |??? x' ?????????? Hsome|];
+      eauto;
+      assert (sub_inst_n x' (add_objs x M' M) M'0)
+        by (apply not_Is_defined_in_eq_EqApp in Hnd;
+            unfold sub_inst_n, sub_inst, add_objs in *; intro;
+            rewrite mfind_inst_gso; auto; intro; subst x; destruct xs;
+            inv Hsome; apply Hnd; now constructor);
+      eauto.
+  Qed.
 
     Theorem correctness:
       forall f xss oss,
@@ -213,14 +366,17 @@ Module Type CORRECTNESS
           (P_equation := fun b H e =>
                            sem_equation G b H e ->
                            exists M mems,
+                             memories_spec M (ps_from_list (map fst mems)) H ->
                              Forall (SemSM.sem_equation P SynSM.Last b H M mems)
                                     (translate_eqn (ps_from_list (map fst mems)) e))
           (P_reset := fun f r xss oss =>
                         sem_reset G f r xss oss ->
-                        True);
+                        exists ma,
+                          (forall n, find_node f G = Some n -> ma = translate_node n)
+                          /\ exists M, SemSM.sem_mode P SynSM.Last ma step M xss oss
+                                 /\ SemSM.sem_mode P (SynSM.Inter 0) ma reset M (fun _ => []) (fun _ => []));
         eauto.
       - repeat (econstructor; eauto).
-        apply caexp_correctness; auto.
 
       - intro Sem; clear Sem.
         destruct IHsem_node as (ma & Spec & M & Sem).
@@ -233,19 +389,37 @@ Module Type CORRECTNESS
         apply find_node_translate in Find as (ma' & ? & Find & E).
         subst.
         simpl.
-        assert (exists y, hd_error x = Some y) as (y & ?).
-        { apply length_hd_error.
-          repeat match goal with H: sem_vars _ _ _ _ |- _ => specialize (H 0); simpl in H end.
-          repeat match goal with H: Forall2 _ _ _ |- _ => apply Forall2_length in H end.
-          match goal with H: length x = _ |- _ => rewrite H end.
-          repeat try match goal with H: _ = ?x |- _ => rewrite <-H end.
-          rewrite map_length; apply n.(n_outgt0).
-        }
-        exists (madd_obj y M (@empty_memory SemSM.mvalues)).
+        (* assert (exists y, hd_error x = Some y) as (y & ?). *)
+        (* { apply length_hd_error. *)
+        (*   repeat match goal with H: sem_vars _ _ _ _ |- _ => specialize (H 0); simpl in H end. *)
+        (*   repeat match goal with H: Forall2 _ _ _ |- _ => apply Forall2_length in H end. *)
+        (*   match goal with H: length x = _ |- _ => rewrite H end. *)
+        (*   repeat try match goal with H: _ = ?x |- _ => rewrite <-H end. *)
+        (*   rewrite map_length; apply n.(n_outgt0). *)
+        (* } *)
+        exists (madd_obj (hd default x) M (@empty_memory SemSM.mvalues)).
         repeat (econstructor; eauto).
         apply mfind_inst_gss.
 
-      - admit.
+      - intro Sem; clear Sem.
+        destruct IHsem_node as (ma & Spec & M & Step & Reset); auto.
+        match goal with H: sem_reset _ _ _ _ _ |- _ => inversion_clear H as [???? Sem] end.
+        simpl.
+        exists (madd_obj (hd default x) M (@empty_memory SemSM.mvalues)).
+        econstructor.
+        pose proof (Sem 0) as Sem0; inv Sem0.
+        edestruct find_node_translate as (ma' & P' & ? & ?); eauto.
+        subst.
+        econstructor.
+        + econstructor; eauto.
+          * intro; eapply SemSM.SNil.
+          * apply mfind_inst_gss.
+          * erewrite <-Spec; eauto.
+          * constructor.
+        + constructor; eauto.
+          econstructor; eauto.
+          * apply mfind_inst_gss.
+          * erewrite <-Spec; eauto.
 
       - intro Sem; clear Sem; simpl.
         exists (madd_mem x {| SemSM.first := xs; SemSM.inter := [] |} (@empty_memory SemSM.mvalues)).
@@ -259,12 +433,14 @@ Module Type CORRECTNESS
           * simpl; intro n.
             match goal with H: xs = _ |- _ => now rewrite H end.
 
+      - admit.
+
       - exists (translate_node n); split; eauto.
         + intros.
           match goal with
           | H: find_node ?f ?G = Some _,
                H': find_node f G = Some _ |- _ => rewrite H in H'; inv H'
           end; auto.
-        +
+        + admit.
 
     Qed.
